StackLean/Shuffle.lean
@@ -1,6 +1,8 @@
 import Init.Data.List
 import Mathlib.Data.Nat.Basic
+import Mathlib.Data.Bool.AllAny
 import Aesop
+import Mathlib.Tactic.Linarith
 
 import StackLean.Definitions
 import StackLean.LSet
@@ -26,6 +28,16 @@ abbrev tail_is_compatible (stack: Stack) (target : Target) : Prop :=
   )
 
 @[simp]
+-- Do we have a sufficient quantity of slot?
+abbrev more_needed_on_stack (stack: Stack) (target : Target) (slot : Slot) : Prop :=
+  stack.total_count slot < target.min_count slot
+
+@[simp]
+-- Are any of the stack args required in the tail but not there yet?
+abbrev any_arg_required_in_tail {hargs : args_is_correct stack target} (stack: Stack) (target : Target) : Prop :=
+  (stack.args target).any (λ arg => more_needed_on_stack stack target arg)
+
+@[simp]
 abbrev input_contains_all_target_vars (input : Stack) (target : Target) : Prop
   := target.vars ⊆ input.vars
 
@@ -41,6 +53,7 @@ def distance (stack : Stack) (target : Target) : ℕ :=
     |> List.sum
 
   let deficit := (Int.ofNat stack.length - Int.ofNat target.size).natAbs
+  -- TODO: use List.diff
   let args_wrong := compare (stack.args target) (target.args.drop (target.size - stack.length))
   let tail_difference := (target.liveOut - (stack.tail_region target).vars).count
 
@@ -54,6 +67,45 @@ inductive ShuffleResult (start : Stack) where
   | ResultStack (finish : Stack) (trace : Trace start finish)
   deriving Repr
 
+theorem args_is_correct_eq (stack : Stack) (target : Target) (hargs : args_is_correct stack target) : stack.args target = target.args := by
+  obtain ⟨hsz, _⟩ := hargs
+  unfold Stack.args
+  split_ifs with h
+  · exfalso; linarith [h, hsz]
+  · apply List.ext_getElem
+    all_goals grind only [= List.length_take, = List.getElem_take, = Nat.min_def]
+
+-- if the args are correct, and at least one arg is still required in the tail,
+-- then target.liveOut.count must be > 0.
+theorem args_correct_required_tail_out_size
+  (stack : Stack) (target : Target)
+  (hargs : args_is_correct stack target) (hreq : any_arg_required_in_tail (hargs := hargs) stack target)
+    : target.liveOut.count > 0
+  := by
+    have ⟨v, ⟨hvmem, hmnv⟩⟩ : ∃ v ∈ (stack.args target), more_needed_on_stack stack target v := by
+      rw [←List.any_iff_exists_prop]; exact hreq
+
+    have : 0 < (stack.args target).count v := by
+      rw [List.count_pos_iff]; exact hvmem
+
+    have : 0 < stack.count v := by
+      grind only [
+        List.take_sublist, usr List.Sublist.length_le, =_ List.contains_iff_mem, usr
+        List.Sublist.count_le, = List.any_eq, usr List.count_le_length, → List.Sublist.subset, =
+        List.count_eq_length_filter, stack_args_sublist_stack
+      ]
+
+    have (s : Slot) : List.count s (stack.args target) = List.count s target.args := by
+      rw [args_is_correct_eq]; unfold args_is_correct; exact hargs
+    have (s : Slot) : List.count s (stack.args target) ≤ List.count s stack := by
+      apply List.Sublist.count_le; apply stack_args_sublist_stack
+
+    have : ∃ v, v ∈ target.liveOut := by
+      simp [more_needed_on_stack, Stack.total_count, Target.min_count] at hmnv
+      cases' v <;> grind only
+
+    exact List.length_pos_iff_exists_mem.mpr this
+
 mutual
 
 -- TODO: target can only be reached from stack if the variable set of target ⊆ the variable set of stack
@@ -62,10 +114,31 @@ def shuffle (stack : Stack) (target : Target) (_ : input_contains_all_target_var
 
 @[simp]
 def shuffle.go (start : Stack) (trace : Trace start state) (target : Target) : ShuffleResult start :=
-  if args_is_correct state target then
-    if tail_is_compatible state target
-    then .ResultStack state trace
-    else .StackTooDeep
+  if hargs : args_is_correct state target then
+    if hreq : any_arg_required_in_tail state target
+    then
+      match (state.args target).reverse.findFinIdx? (more_needed_on_stack state target) with
+      -- we already validated that at least one arg is required in hreq
+      | none => .ForbiddenState
+      --
+      | some elem_idx =>
+        if hidx : elem_idx.val > 15 then
+          .StackTooDeep
+        else
+          -- utility lemmas
+          have : (state.args target).length = target.args.length := by simp_all; grind only
+          have : 0 < target.liveOut.count := args_correct_required_tail_out_size state target hargs hreq
+          have : target.args.length + target.liveOut.count ≤ target.size := target.size.property
+          have : target.args.length < state.length := by omega
+          have : elem_idx < (state.args target).length := (Fin.cast List.length_reverse elem_idx).isLt
+
+          -- termination
+          have : distance (state[elem_idx] :: state) target < distance state target := by sorry
+
+          -- dup and recurse
+          shuffle.go start (.Dup (elem_idx + 1) (by omega) (by omega) (by omega) trace) target
+    else
+      .ResultStack state trace
 
   -- if we have too much stuff
   else if hlen : state.length > target.size then
@@ -74,7 +147,9 @@ def shuffle.go (start : Stack) (trace : Trace start state) (target : Target) : S
 
       -- pop always decreases the distance
       have : distance (List.tail state) target < distance state target := by
-        simp_all [distance]; split_ifs with hsz <;> refine Nat.lt_of_add_lt_add_right _
+        simp_all [distance]; split_ifs with hsz
+        · refine Nat.lt_of_add_lt_add_right _
+        · refine Nat.lt_of_add_lt_add_right _
 
       -- apply the pop and recurse
       shuffle.go start (.Pop (by grind) trace) target
